feat: updated the headers

diffie_hellman.v
@@ -1,1 +1,60 @@
-(*** Prova de Completude do Algorítmo de Criptografia Diffie Hellman ***)
+(*** Completeness proof for Diffie Hellma(DH)n Algorithm ***)
+(*** To proof it we must first proof that ***)
+
+Require export Coq.ZArith.Zdiv.
+
+(*** 
+    DH algorithm works basic as an Alice and Bob communication and they
+    have some important numbers, they are:
+    
+    Alice's PublicKey, Bob's PublicKey
+    Alice's PrivateKey, Bob's PrivateKey
+    
+    Those keys are used to compute the final key with the equation:
+    
+    SharedSeed = g^
+***)
+
+
+
+(*** Helper functions****)
+Fixpoint isEqual (a: String) (b: String) : Bool
+
+(** DH Functions **)
+Fixpoint modExp (b : nat) (e : nat) (m : nat): nat.
+
+Fixpoint calculatePublicKey (private_k : nat, base : nat, gen : nat) : nat.
+
+Fixpoint calculateSharedSeed (private_k : nat, public_k : nat, base : nat, gen : nat) : nat.
+
+Fixpoint caesarCrypt (seed : .nat, msg_toSend: String) : String.
+
+Fixpoint caesarDecript (seed : .nat, msg_received: String) : String.
+
+
+(*** Extra: Proof for any symmetric encryption ***)
+Fixpoint symmetricCrypt (seed : .nat, msg_toSend: String) : String.
+
+Fixpoint symmetricDecript (seed : .nat, msg_received: String) : String.
+
+(*** Extra: Proof for any symmetric encryption ***)
+
+Theorem equalKeys:
+    forall (private_k1:nat) (private_k2:nat) (gen:nat) (base:nat), 
+    calculateSharedSeed(private_k1, calculatePublicKey(private_k2, base, gen), base, gen) = calculateSharedSeed(private_k2, calculatePublicKey(private_k1, base, gen), base, gen) 
+
+Theorem DHCorrect:
+    forall message:String, (symmetricDecript( symmetricCrypt (message) )) = message
+
+
+Theorem Encrypt_Complete: 
+    forall message: String, caesarCrypt message
+
+(*** https://github.com/coq-contribs/rsa/blob/master/Rsa.v ***)
+
+
+(*** Extras: Rationalize over DiffieHellman protocol implementations using 
+Protocol Composition Logic, as defined in this paper from stanford university:
+http://seclab.stanford.edu/pcl/papers/rdm-tgc07.pdf ***)
+
+
